Cvc/Srt/Extra.lean
@@ -1,5 +1,152 @@
-import Cvc.Srt.SrtBij
+/-
+Copyright (c) 2023-2025 by the authors listed in the file AUTHORS and their
+institutional affiliations. All rights reserved.
+Released under Apache 2.0 license as described in the file LICENSE.
+Authors: Adrien Champion
+-/
+
+import Cvc.Srt.Defs
+import Cvc.Srt.Types
 
 
 
+/-! # Relates `Srt`-s to `Type`-s
+
+Main class `IsSrt (α : Type)` associates `srt : Srt` to `α`. It guarantees this association works
+both ways by asking for a proof that `α = srt.toType`.
+-/
 namespace Cvc
+
+
+
+/-- Provides a `srt : Srt` such that `α = srt.toType`. -/
+class IsSrt (α : Type) where mk ::
+  /-- `Srt` version of `α`. -/
+  srt : Srt
+  /-- Turning `srt` into a `Type` results in `α`. -/
+  h_bij : α = srt := by
+    simp [Cvc.Srt.toType, IsSrt.h_bij, *] <;> rfl
+
+/-- Retrieves the `Srt` corresponding to a `Type`. -/
+abbrev getSrt (α : Type) [I : IsSrt α] : Srt :=
+  I.srt
+
+namespace Srt
+
+instance instIsSrt (srt : Srt) : IsSrt srt := { srt }
+
+@[inherit_doc getSrt]
+abbrev ofType := Cvc.getSrt
+
+@[simp]
+theorem toType_ofType (α : Type) [I : IsSrt α] : ofType α = α := by
+  let {srt, h_bij} := I
+  cases h_bij
+  cases srt <;> rfl
+
+@[simp]
+theorem ofType_toType (srt : Srt) : ofType srt = srt := by
+  cases srt <;> rfl
+
+end Srt
+
+namespace IsSrt
+
+/-! ## Instances for simple types -/
+
+instance instUnit : IsSrt Unit := mk .unit
+instance instBool : IsSrt Bool := mk .bool
+instance instInt : IsSrt Int := mk .int
+instance instRat : IsSrt Rat := mk .real
+instance instString : IsSrt String := mk .string
+instance instRoundingMode : IsSrt Cvc.RoundingMode := mk <| .roundingMode
+instance instRegex : IsSrt Cvc.Regex := mk <| .regex
+
+/-! ## Instances for non-`Srt`-parameterized types -/
+instance instAnyFloat : IsSrt (Cvc.AnyFloat exp sig) := mk <| .float exp sig
+instance instAbstract : IsSrt (Cvc.Abstract k) := mk <| .abstract k
+instance instFiniteField : IsSrt (Cvc.FiniteField n) := mk <| .finiteField n
+instance instBitVec : IsSrt (BitVec size) := mk <| .bitVec size
+instance instUninterpreted : IsSrt (Uninterpreted name) := mk <| .uninterpreted name
+
+/-! ## Instances composite types -/
+section variable [A : IsSrt α] [B : IsSrt β]
+
+instance instArray : IsSrt (Array α) := mk <| .seq A.srt
+instance instFunction : IsSrt (α → β) := mk <| .function A.srt B.srt
+instance instProd : IsSrt (α × β) := mk <| .prod A.srt B.srt
+instance instTMap : IsSrt (Cvc.TMap α β) := mk <| .array A.srt B.srt
+instance instBag : IsSrt (Cvc.Bag α) := mk <| .bag A.srt
+instance instSet : IsSrt (Cvc.Set α) := mk <| .set A.srt
+
+end
+
+end IsSrt
+
+
+
+/-! ## Refinement of `IsSrt` to arithmetic sorts -/
+
+/-- Proof that the sort associated to `α` is arithmetic. -/
+protected abbrev is_arith (α : Type) [IsSrt α] :=
+  Srt.ofType α |>.is_arith
+
+instance [IsSrt α] : Decidable (Cvc.is_arith α) := by
+  simp only [Cvc.is_arith, Srt.is_arith, Srt.isArith, Srt.ofType, getSrt]
+  cases IsSrt.srt α <;> (
+    simp
+    try exact instDecidableFalse
+    try exact instDecidableTrue
+  )
+
+@[simp]
+theorem is_arith_def (α : Type) [inst : IsSrt α] : Cvc.is_arith α → (α = Int ∨ α = Rat) := by
+  let {srt, h_bij} := inst
+  cases h_bij
+  cases srt <;> simp
+
+def is_arith_srt_def (α : Type) [inst : IsSrt α]
+: Cvc.is_arith α → (inst.srt = .int ∨ inst.srt = .real) := by
+  let {srt, h_bij} := inst
+  cases h_bij
+  cases srt <;> simp
+
+namespace IsSrt
+
+/-- Extends `IsSrt` with a proof that `α`'s `Srt` is arithmetic. -/
+protected class Arith (α : Type) extends toIsSrt : IsSrt α where
+  /-- Sort `srt` is an arithmetic sort. -/
+  h_arith : Cvc.is_arith α := by simp
+
+namespace Arith
+
+example [IsSrt.Arith α] : IsSrt α := inferInstance
+
+/-! ## Instances for `Int` and `Rat` (`Real`) -/
+instance instInt : IsSrt.Arith Int := {}
+instance instRat : IsSrt.Arith Rat := {}
+
+theorem int_or_rat (α : Type) [inst : IsSrt.Arith α] : α = Int ∨ α = Rat :=
+  Cvc.is_arith_def α inst.h_arith
+
+def int_or_rat' (α : Type) [inst : IsSrt.Arith α] : inst.srt = .int ∨ inst.srt = .real :=
+  Cvc.is_arith_srt_def α inst.h_arith
+
+def inspect' (α : Type) [inst : IsSrt.Arith α]
+  (fInt : (h : α = Int) → β) (fRat : (h : α = Rat) → β)
+: β :=
+  let { toIsSrt, h_arith } := inst
+  let { srt, h_bij } := toIsSrt
+  by
+    cases inst.int_or_rat
+    case inl => apply fInt ; assumption
+    case inr => apply fRat ; assumption
+
+def inspect {α : Type} {β : Sort u} [inst : IsSrt.Arith α]
+  (fInt : (h : inst.srt = .int) → β) (fRat : (h : inst.srt = .real) → β)
+: β :=
+  inst.int_or_rat'.by_cases fInt fRat
+
+end Arith
+
+end IsSrt
